about t pull?

basic_types.v
@@ -3,13 +3,18 @@ Require Import ssreflect.
 From mathcomp Require Import ssreflect seq ssrnat.
 From istari Require Import Sigma Tactics
      Syntax Subst SimpSub Promote Hygiene
-     ContextHygiene Equivalence Rules Defined.
+     ContextHygiene Equivalence Equivalences Rules Defined lemmas0 derived_rules.
 
-Definition oof M A: (@Syntax.judgement obj) := deq M M A.
-
-Definition oof_t M: (@Syntax.judgement obj) := deqtype M M.
 
 Definition U0 : (term obj) := univ nzero.
+
+Lemma nat_U0: forall G,
+    tr G (oof nattp U0). Admitted.
+Hint Resolve nat_U0. 
+
+Lemma nat_type: forall G,
+      tr G (deqtype nattp nattp). Admitted.
+Hint Resolve nat_type. 
 
 Definition leq_t n m : term obj :=
   app (app leqtp n) m.
@@ -35,11 +40,6 @@ Lemma lt_type: forall G n1 n2,
     tr G (oof (ltpagetp n1 n2) U0).
   Admitted.
 
-Lemma nat_U0: forall G,
-    tr G (oof nattp U0). Admitted.
-
-Lemma nat_type: forall G,
-      tr G (deqtype nattp nattp). Admitted.
 
 Lemma U0_type: forall G,
     tr G (deqtype U0 U0). Admitted.
@@ -47,6 +47,10 @@ Lemma U0_type: forall G,
 Hint Resolve nat_type nat_U0 zero_typed leq_refl leq_type lt_type U0_type.
 
 Definition if_z (n: term obj): (term obj) := ppi1 n.
+
+
+Lemma if_z_typed n G : tr G (oof n nattp) -> tr G (oof (if_z n) booltp).
+Admitted.
 
 (*n - m*)
 Definition minusbc: (term obj) := lam
@@ -88,28 +92,99 @@ Lemma nsucc_lt: forall G n, tr G (oof n nattp) ->
                        tr G (oof triv (lt_t n (nsucc n))).
 Admitted.
 
+Definition eq_b n1 := app (wind (lam (* x = 0*)
+                             (lam (*x = 1, y= 0*)
+                                ( lam
+                                    ( (*x = 2, y = 1, z = 0*)
+                                      bite (var 2)
+                                           (lam (*x = 3, y = 2, z = 1, n2 = 0*)
+                                              (if_z (var 0))
+                                           ) (*first one is zero*)
+                                           ( (*first one is nonzero*)
+                                             lam
+                                               ( (*x = 3, y = 2, z = 1, n2 = 0*)
+                                                 bite (if_z (var 0))
+                                                      bfalse
+                                                      (app (app (var 1) triv) (app (ppi2 (var 0)) triv))
+                                               )
+                                           )
+                                    )
+                                )
+                             )                           
+                          )) n1.
 
-Definition eq_bbc: (term obj) := lam
-                         (
-                           (*f := 0*)
-                           lam ( (*f:= 1, n := 0*)
-                               lam ((*f := 2, n:= 1, m := 0*)
-                                   let f := (var 2) in
-                                   let n := (var 1) in
-                                   let m := (var 0) in
-                                                  bite (if_z n)
-                                                  (if_z m)
-                                                  (bite (if_z m)
-                                                     (bfalse)
-                                                    (app (app f (app (ppi2 n) triv)) (app (ppi2 m) triv)))
-                                                  ))).
- Definition eq_b: (term obj) := app theta eq_bbc.
+Lemma subst_nat: forall s,
+    @ subst obj s nattp = nattp.
+  intros. unfold nattp. auto. Qed.
 
-Lemma eqb_typed {G}: tr G (oof eq_b (arrow nattp (arrow nattp booltp))).
+Hint Rewrite subst_nat: core subst1.
+
+Ltac weaken H := eapply tr_formation_weaken; apply H.
+Ltac var_solv0 := try (apply tr_hyp_tm; repeat constructor).
+
+Hint Rewrite subst_nat: core subst1.
+
+Ltac var_solv' := unfold oof; match goal with |- tr ?G' (deq (var ?n) ?n' ?T) => try
+                                 rewrite - (subst_nat (sh (n.+1))); var_solv0 end.
+
+Lemma w_elim_hyp G1 G2 a b J :
+      tr (G2 ++ hyp_tm (sigma a (arrow b (subst sh1 (wt a b)))) :: G1) J
+      -> tr (G2 ++ hyp_tm (wt a b) :: G1) J.
+  Admitted.
+
+           Lemma eqb_typed {G} n1:
+  tr G (oof n1 nattp) ->
+  tr G (oof (eq_b n1) (arrow nattp booltp)).
+  intros.
+  change (arrow nattp booltp) with (subst1 n1 (arrow nattp booltp)).
+  apply (tr_wt_elim _ booltp (bite (var 0) voidtp unittp)).
+  - assumption.
+  - simpsub. simpl.
+    rewrite make_app2.
+    change (lam (if_z (var 0))) with
+      (subst (under 2 sh1)  (lam (if_z (var 0)))).
+    change (lam
+             (bite (if_z (var 0)) bfalse
+                (app (app (var 1) triv)
+                     (app (ppi2 (var 0)) triv)))) with
+        (subst (under 2 sh1)
+(lam (bite (if_z (var 0)) bfalse
+                (app (app (var 1) triv)
+                     (app (ppi2 (var 0)) triv))))
+        ).
+    apply tr_booltp_eta_hyp; simpsub; simpl; simpsub; rewrite ! subst_nat;
+      apply tr_arrow_intro; auto; try weaken tr_booltp_formation.
+    + apply if_z_typed. var_solv'.
+    + apply (w_elim_hyp _ [::]). match goal with |- tr ?G (deq ?M ?M ?A) => change M with
+       (@subst obj (under 0 (dot (ppi2 (var 0)) (dot (ppi1 (var 0)) sh1)))
+       (bite (var 1) bfalse
+          (app (app (var 2) triv)
+               (app (var 0) triv)))) end.
+      apply tr_sigma_eta_hyp.
+      simpsub. simpl.
+          change (app (app (var 2) triv)
+                      (app (var 0) triv)) with
+              (@subst obj (under 1 sh1)
+                     (app (app (var 1) triv)
+                          (app (var 0) triv))).
+          change bfalse with (@subst obj (under 1 sh1) bfalse).
+          rewrite make_app1.
+          apply tr_booltp_eta_hyp; simpsub.
+      * constructor.
+      * eapply tr_compute_hyp.
+        {
+          constructor. apply equiv_pi. apply reduce_equiv.
+          apply reduce_bite_beta2. apply reduce_id.
+          apply equiv_refl.
+        }
+
+              )
+
+           )
 Admitted.
 
 Lemma eqapp_typed G m n: tr G (oof m nattp) -> tr G (oof n nattp) ->
-  tr G (oof (app (app eq_b m) n) booltp). Admitted.
+  tr G (oof (app (eq_b m) n) booltp). Admitted.
 
 Lemma eqb_P G n m : tr G (oof n nattp) ->
                     tr G (oof m nattp) ->
@@ -119,23 +194,3 @@ Lemma eqb_P G n m : tr G (oof n nattp) ->
 Admitted.
 
 
-Definition eq_wind = wind (lam (* x = 0*)
-                             (lam (*x = 1, y= 0*)
-                                ( lam
-                                    ( (*x = 2, y = 1, z = 0*)
-                                      bite x
-                                           (lam (*x = 3, y = 2, z = 1, n2 = 0*)
-                                              (if_z (var 0))
-                                           ) (*first one is zero*)
-                                           ( (*first one is nonzero*)
-                                             lam
-                                               ( (*x = 3, y = 2, z = 1, n2 = 0*)
-                                                 bite (if_z (var 0))
-                                                      false
-                                                      (z * (ppi2 (var 0)) *)
-                                               )
-                                           )
-                                    )
-                                )
-                             )                           
-                          )
